expose the whole goal to the split_sepclause search tactic
so that it can context-match on a `length` precondition to
get the length desired by the callee, so we don't need
`with_len` any more.

Also switch from `seps [...; emp (continuation)]` to
`seps [...] /\ continutation`, adapting all cancellation
lemmas to a goal of shape `seps [...] /\ continuation`
instead of `seps [...]`, and then use continutation:=True
if there is none.
Adapting the cancellation infrastructure to include
`_ /\ continuation` everywhere is a bit of a disadvantage,
but has the advantage that split_sepclause search hints
can identify the continuation (which might be of shape
`more_sideconditions /\ actual_continutation`) without
having to iterate to the last element of the `seps`,
so the context match on `more_sideconditions` to find
a `length ?vs = desired_length` can focus more easily
on just the part where we expect to find the length
equality.

Moreover, in LiveVerif, use get_option wrapped around
Memory.load/Memory.store as preconditions of wp_load/store
instead of inlined separation logic preconditions, so
that automation can check more easily whether we're solving
a load sidecondition or a store sidecondition, because the
former requires clearing the split_merge_lemma stack without
using it, whereas the latter requires applying all the merges.

bedrock2/src/bedrock2/SepCalls.v
@@ -41,52 +41,68 @@ Section SepLog.
   Context {width: Z} {word: word.word width} {mem: map.map word byte}.
   Context {word_ok: word.ok word} {mem_ok: map.ok mem}.
 
-  (* Hides a sep behind a definition so that flattening operations keep
-     memPred and its associated purePred together as one clause *)
-  Definition with_pure(memPred: mem -> Prop)(purePred: Prop): mem -> Prop :=
-    sep memPred (emp purePred).
+  Lemma icancel_start: forall (P Q: Tree.Tree (mem -> Prop)) (C: Prop) (m: mem),
+      Tree.to_sep P m ->
+      impl1 (seps (Tree.flatten P)) (seps (Tree.flatten Q)) /\ C ->
+      Tree.to_sep Q m /\ C.
+  Proof.
+    intros * ? (? & ?). split. 2: assumption.
+    eapply Tree.impl1_to_sep_of_impl1_flatten in H0.
+    apply H0. assumption.
+  Qed.
 
   (* R, typically instantiated to `seps [whatever; is; left]`, appears twice:
      On the left of the impl1 (this determines its value), and as the first
-     element of the `seps` on the right (there, it is an evar for the frame).
-     P is the continuation postcondition. *)
-  Lemma impl1_done: forall (R: mem -> Prop) (P: Prop),
-      P -> impl1 R (seps [R; emp P]).
+     element of the `seps` on the right (there, it is an evar for the frame). *)
+  Lemma icancel_done_evar_r: forall (R: mem -> Prop) (C: Prop),
+      C -> impl1 R (seps [R]) /\ C.
   Proof.
-    unfold impl1, seps. intros. apply sep_emp_r. auto.
+    unfold impl1, seps. auto.
   Qed.
 
-  (* All arguments except stmt are just ghost parameters to guide typeclass search.
+  Lemma icancel_done_nil_r: forall (C: Prop),
+      C -> impl1 (seps (map := mem) []) (seps []) /\ C.
+  Proof. split. 2: assumption. exact impl1_refl. Qed.
+
+  (* On goals of this shape, `typeclasses eauto with split_speclause_goal` will be called,
+     which will pose its result `stmt` as a hypothesis and then shelve the goal.
      The shape of stmt has to be
        forall valAll valPart valFrame1 ... valFrameN,
          sidecondition saying that assembling valPart valFrame1 ... valFrameN = valAll ->
          iff1 (predAll valAll addrAll) (sep (predPart valPart addrPart)
                                             (seps [Frame...]))
-     but since that's a variable number of universally quantified variables, it would
-     be a bit cumbersome to enforce that shape in Gallina, so we don't.
      Note that stmt needs to be not only applicable to split oldAll into oldPart and a
      frame, but also to merge back a newPart and newFrame (potentially modified as well,
      eg if a function separately takes two record fields) into a newAll.
      So stmt needs to be more general than oldAll/oldPart.
-     But we still pass in the specific oldPart so that typeclass search for split_sepclause
-     can determine its length, either from a with_len, or by computing it.
      The specific shape of the RHS of the above iff1 is for compatibility with
      cancel_part_of_ith_lhs_with_first_rhs, so that no sep flattening is required
      during cancellation. *)
-  Definition split_sepclause(oldAll oldPart: mem -> Prop)(stmt: Prop) := stmt.
+  Definition split_sepclause(oldAll oldPart: mem -> Prop)(oldFrame: list (mem -> Prop))
+             (remainingGoal: Prop) :=
+    iff1 oldAll (sep oldPart (seps oldFrame)) /\ remainingGoal.
 
   Let nth n xs := SeparationLogic.hd (emp(map:=mem) True) (SeparationLogic.skipn n xs).
   Let remove_nth n (xs : list (mem -> Prop)) :=
         (SeparationLogic.app (SeparationLogic.firstn n xs)
                              (SeparationLogic.tl (SeparationLogic.skipn n xs))).
 
-  Lemma cancel_part_of_ith_lhs_with_first_rhs: forall i Ls Li Frame R1 Rs,
-      nth i Ls = Li ->
-      iff1 Li (sep R1 (seps Frame)) /\
-      impl1 (seps (SeparationLogic.app (remove_nth i Ls) Frame)) (seps Rs) ->
-      impl1 (seps Ls) (seps (R1 :: Rs)).
+  Lemma cancel_ith_lhs_with_first_rhs: forall i Ls R1 Rs C,
+      impl1 (nth i Ls) R1 ->
+      impl1 (seps (remove_nth i Ls)) (seps Rs) /\ C ->
+      impl1 (seps Ls) (seps (R1 :: Rs)) /\ C.
   Proof.
-    intros. destruct H0. subst Li.
+    intros * ? (? & ?). split. 2: assumption.
+    eapply (cancel_seps_at_indices_by_implication i 0%nat); eassumption.
+  Qed.
+
+  Lemma cancel_part_of_ith_lhs_with_first_rhs: forall i Ls Li Frame R1 Rs C,
+      nth i Ls = Li ->
+      split_sepclause Li R1 Frame
+         (impl1 (seps (SeparationLogic.app (remove_nth i Ls) Frame)) (seps Rs) /\ C) ->
+      impl1 (seps Ls) (seps (R1 :: Rs)) /\ C.
+  Proof.
+    intros. destruct H0 as (?&?&?). subst Li. split. 2: assumption.
     unfold nth, remove_nth in *.
     rewrite <-(seps_nth_to_head i Ls).
     rewrite H0.
@@ -97,37 +113,24 @@ Section SepLog.
     etransitivity. 2: eassumption.
     ecancel.
   Qed.
-
-  (* Transforms the goal so that goal modifications that are made while proving Rs
-     are still visible when proving the continuation Cont of the program *)
-  Lemma put_and_r_into_emp_sep: forall (Cont: Prop) (R: mem -> Prop) (m: mem),
-      sep R (emp Cont) m ->
-      R m /\ Cont.
-  Proof. intros. eapply sep_emp_r. exact H. Qed.
 End SepLog.
 
-(* Hints for `(split_sepclause ?oldAll ?oldPart ?stmt)` goals *)
+Definition split_merge_lemma(P: Prop) := P.
+
+(* Hints for `(split_sepclause ?oldAll ?oldPart ?oldFrame ?remainginGoal)` goals *)
 Create HintDb split_sepclause_goal.
 #[global] Hint Opaque split_sepclause : split_sepclause_goal.
 
-Ltac default_solve_split_sepclause_goal_or_else error_handler :=
-  first [ once (typeclasses eauto with split_sepclause_goal)
-        (* `typeclasses eauto` instead of eauto because eauto unfolds split_sepclause
-           and then just does `exact H` for the last Prop in the context, and it
-           seems that `Hint Opaque` and `Hint Constants Opaque` don't fix that
-           (and `Opaque split_sepclause` would fix it, but also affects the conversion
-           algorithm).
-           `once` because otherwise later errors will cause `typeclasses eauto` (which
-           is multisuccess) to backtrack, and the error will not be the later error,
-           but a generic "Tactic failure: Proof search failed." from `typeclasses eauto` *)
+Ltac default_pose_split_merge_lemma_or_else error_handler :=
+  first [ unshelve (solve [eauto with split_sepclause_goal])
         | error_handler Error:("This goal should be solvable by"
-                               "typeclasses eauto with split_sepclause_goal") ].
+                               "eauto with split_sepclause_goal") ].
 
 (* Hook that can be overriden with ::=, for users who don't want to use the
    split_sepclause_goal hint DB.
    In case of failure, should call error_handler with one argument of type tactic_error *)
-Ltac solve_split_sepclause_goal_or_else error_handler :=
-  default_solve_split_sepclause_goal_or_else error_handler.
+Ltac pose_split_merge_lemma_or_else error_handler :=
+  default_pose_split_merge_lemma_or_else error_handler.
 
 
 (* Hints to solve the sideconditions of the `stmt` above, when using the iff1
@@ -159,96 +162,104 @@ Ltac default_solve_merge_sepclause_sidecond_or_pose_err :=
 Ltac solve_merge_sepclause_sidecond_or_pose_err :=
   default_solve_merge_sepclause_sidecond_or_pose_err.
 
-Ltac split_ith_left_to_cancel_with_fst_right0 i are_you_sure_about_i :=
+Ltac split_ith_left_and_cancel_with_fst_right0 i are_you_sure_about_i :=
+  eapply (cancel_part_of_ith_lhs_with_first_rhs i);
+  cbn [SeparationLogic.hd SeparationLogic.tl
+       SeparationLogic.app SeparationLogic.firstn SeparationLogic.skipn];
+  [ reflexivity | ];
+  pose_split_merge_lemma_or_else
+    ltac:(fun e => lazymatch are_you_sure_about_i with
+                   | true => pose_err e
+                   | false => fail
+                   | _ => fail 10000 "argument are_you_sure_about_i should be a bool"
+                   end);
   lazymatch goal with
-  | |- Lift1Prop.impl1 (seps ?L) (seps (?RHead :: ?RRest)) =>
-    eapply (cancel_part_of_ith_lhs_with_first_rhs i L);
-    cbn [SeparationLogic.hd SeparationLogic.tl
-         SeparationLogic.app SeparationLogic.firstn SeparationLogic.skipn];
-    [ reflexivity | ];
-    (* Current goal is a conjunction of two subgoals:
-       - iff1 for left-to-right-rewrite that we'll derive from a split_sepclause instance
-       - new impl1 to be proven after this cancellation step *)
-    let Li := lazymatch goal with |- iff1 ?Li _ /\ impl1 _ _ => Li end in
-    let Sp := fresh "Sp" in
-    eassert (split_sepclause Li RHead _) as Sp;
-    [ solve_split_sepclause_goal_or_else
-        ltac:(fun e => lazymatch are_you_sure_about_i with
-                       | true => pose_err e
-                       | false => fail
-                       | _ => fail 10000 "argument are_you_sure_about_i should be a bool"
-                       end)
-    | split;
-    [ lazymatch type of Sp with
-      | split_sepclause _ _ ?stmt =>
-          tryif is_evar stmt then
-            idtac (* debugging and typeclasses eauto above failed *)
-          else (
-            tryif (assert_fails (idtac;
-                     lazymatch ret_type stmt with
-                     | iff1 ?predAll (sep ?predPart (seps ?Frame)) => idtac
-                     end))
-            then pose_err Error:("The conclusion of" Sp "is not of shape"
+  | _: tactic_error _ |- _ => idtac
+  | Sp: ?stmt |- _ =>
+      tryif (assert_fails (idtac;
+                           lazymatch ret_type stmt with
+                           | iff1 ?predAll (sep ?predPart (seps ?Frame)) => idtac
+                           end))
+      then pose_err Error:("The conclusion of" Sp "is not of shape"
                                  "iff1 ?predAll (sep ?predPart (seps ?Frame))")
-            else (
-              cbv [split_sepclause] in Sp;
-              eapply Sp;
-              (* sideconditions of Sp can be left unsolved for debugging *)
-              solve_split_sepclause_sidecond_or_pose_err
-            )
-          )
-      end
-    | (* this goal is the remaining impl1 after cancellation, and it's the only
-         goal supposed to remain open unless debugging *) ] ]
+      else (
+        split; (* also unfolds split_sepclause *)
+        [ eapply Sp;
+          (* sideconditions of Sp can be left unsolved for debugging *)
+          solve_split_sepclause_sidecond_or_pose_err
+        | change (split_merge_lemma stmt) in Sp
+          (* this goal is the remaining (impl1 _ _ /\ _) after cancellation, and it's the
+             only goal supposed to remain open unless debugging *) ]
+      )
   end.
 
 (* Can be called manually to debug *)
-Ltac split_ith_left_to_cancel_with_fst_right i :=
-  split_ith_left_to_cancel_with_fst_right0 i true.
+Ltac split_ith_left_and_cancel_with_fst_right i :=
+  split_ith_left_and_cancel_with_fst_right0 i true.
 
 (* Poses split_sepclause lemmas as hypotheses in the context, forming a stack of
    rewrite steps that have been performed, which can later be undone by
    pop_split_sepclause_stack *)
 Ltac impl_ecancel_step_with_splitting :=
   lazymatch goal with
-  | |- Lift1Prop.impl1 (seps ?L) _ =>
+  | |- impl1 (seps ?L) _ /\ _ =>
     let iLi := index_and_element_of L in (* <-- multi-success! *)
     let i := lazymatch iLi with (?i, _) => i end in
-    split_ith_left_to_cancel_with_fst_right0 i false; []
+    split_ith_left_and_cancel_with_fst_right0 i false; []
+  end.
+
+Ltac impl_ecancel_step_without_splitting :=
+  lazymatch goal with
+  | |- impl1 (seps ?L) (seps (?R1 :: ?Rs))  /\ _ =>
+    assert_fails (idtac; let y := rdelta_var R1 in is_evar y);
+    let iLi := index_and_element_of L in (* <-- multi-success! *)
+    let i := lazymatch iLi with (?i, _) => i end in
+    eapply (cancel_ith_lhs_with_first_rhs i L);
+    cbn [SeparationLogic.hd SeparationLogic.tl
+         SeparationLogic.app SeparationLogic.firstn SeparationLogic.skipn];
+    [solve [auto 1 with nocore ecancel_impl]|]
   end.
 
 Ltac use_sep_asm :=
+  lazymatch goal with
+  | |- _ _ /\ _ => idtac
+  (* to make sure this cancellation code can also be used when there's no continutation
+     postcondition, eg at the end of a proof where we just prove that the computed
+     postcondition implies the desired postcondition *)
+  | |- _ => refine (proj1 (_: _ /\ True))
+  end;
   match goal with
-  | H: sep _ _ ?m |- _ ?m =>
-    refine (Morphisms.subrelation_refl Lift1Prop.impl1 _ _ _ m H)
+  | H: ?P ?m |- ?Q ?m /\ ?C =>
+      let treeP := reify P in
+      let treeQ := reify Q in
+      change (Tree.to_sep treeQ m /\ C);
+      eapply (icancel_start treeP treeQ C);
+      [ cbn [Tree.to_sep]; exact H | cbn [Tree.flatten Tree.interp SeparationLogic.app] ]
   end.
 
 Ltac impl_ecancel :=
-  cancel;
-  repeat (repeat (once ecancel_step_by_implication); try impl_ecancel_step_with_splitting).
+  repeat (impl_ecancel_step_without_splitting || impl_ecancel_step_with_splitting).
 
 Ltac finish_impl_ecancel :=
-  match goal with
-  | |- impl1 ?R (seps [?E; emp ?P]) => is_evar E; refine (impl1_done R P _)
-  | |- impl1 ?x (seps [?E]) => is_evar E; change (impl1 x E); exact impl1_refl
-  | |- impl1 ?x ?y => first [ is_evar x | is_evar y | constr_eq x y ]; exact impl1_refl
-  | |- _ => pose_err Error:("impl_ecancel should cancel all clauses of this goal (except maybe one remaining emp)")
+  lazymatch goal with
+  | |- impl1 ?R (seps [?E]) /\ ?C => is_evar E; refine (icancel_done_evar_r R C _)
+  | |- impl1 (seps []) (seps []) /\ ?C => refine (icancel_done_nil_r C _)
+  | |- _ => pose_err Error:("impl_ecancel should cancel all clauses of this goal")
+  end;
+  lazymatch goal with
+  | |- True => exact I
+  | |- _ => idtac
   end.
-
-Ltac impl_ecancel_assumption :=
-  use_sep_asm;
-  impl_ecancel;
-  try finish_impl_ecancel.
 
 Ltac clear_split_sepclause_stack :=
   repeat match goal with
-         | H: split_sepclause _ _ _ |- _ => clear H
+         | H: split_merge_lemma _ |- _ => clear H
          end.
 
 Ltac pop_split_sepclause_stack_step m :=
   let H := lazymatch goal with H: _ ?m |- _ => H end in
-  let Sp := lazymatch goal with Sp: split_sepclause _ _ _ |- _ => Sp end in
-  cbv [split_sepclause] in Sp;
+  let Sp := lazymatch goal with Sp: split_merge_lemma _ |- _ => Sp end in
+  cbv [split_merge_lemma] in Sp;
   cbn [seps] in Sp, H;
   first [ seprewrite_in (symmetry! Sp) H;
           [ solve_merge_sepclause_sidecond_or_pose_err .. | clear Sp ]
@@ -276,13 +287,6 @@ Ltac intro_new_mem :=
       pop_split_sepclause_stack mNew
   end.
 
-Ltac put_cont_into_emp_sep :=
-  lazymatch goal with
-  | |- sep _ _ ?mOld /\ ?Cont =>
-      apply put_and_r_into_emp_sep
-  | |- _ => fail 10000 "Expected a goal of the form" "(sep _ _ ?mOld /\ ?Cont)"
-  end.
-
 (* ecancel an assumption (using impl1), and also split sepclauses on the left
    while canceling *)
 Ltac scancel_asm :=
@@ -292,5 +296,3 @@ Ltac scancel_asm :=
   | H: tactic_error _ |- _ => idtac
   | |- _ => finish_impl_ecancel
   end.
-
-Ltac after_sep_call := put_cont_into_emp_sep; scancel_asm.
