bedrock2/src/bedrock2/SepAutoArray.v
@@ -6,36 +6,9 @@ Require Import bedrock2.groundcbv.
 Require Import coqutil.Word.Bitwidth.
 Require Import coqutil.Tactics.rewr.
 
-Definition with_len{width}{word: word width}{mem: map.map word byte}{V: Type}
-  (n: nat)(array_pred: sep_predicate mem (list V)): sep_predicate mem (list V) :=
-  fun (a: word) (vs: list V) => with_pure (sepcl array_pred vs a) (List.length vs = n).
-
 Section SepLog.
   Context {width: Z} {BW: Bitwidth width} {word: word.word width} {mem: map.map word byte}.
   Context {word_ok: word.ok word} {mem_ok: map.ok mem}.
-
-  Lemma with_len_eq[V: Type]: forall (array_pred: sep_predicate mem (list V)) vs n,
-      List.length vs = n ->
-      sepcl (with_len n array_pred) vs = sepcl array_pred vs.
-  Proof.
-    intros. unfold with_len, with_pure, sepcl. extensionality a.
-    replace (List.length vs = n) with True.
-    - eapply iff1ToEq. cancel.
-    - apply propositional_extensionality. split; auto.
-  Qed.
-
-  Lemma extract_pure: forall (P: Prop) (R1 R2: mem -> Prop) m,
-      sep (with_pure R1 P) R2 m -> P.
-  Proof.
-    unfold with_pure, sep, emp. intros. fwd. assumption.
-  Qed.
-
-  Lemma extract_with_len[V: Type]:
-    forall [array_pred: sep_predicate mem (list V)] [vs n m R a],
-      sep (a :-> vs : with_len n array_pred) R m -> List.length vs = n.
-  Proof.
-    intros. eapply extract_pure in H. exact H.
-  Qed.
 
   Lemma array_app{E : Type}{elem: sep_predicate mem E}{sz: Z}:
     forall (xs ys: list E) (start : word),
@@ -57,23 +30,21 @@ Section SepLog.
     reflexivity.
   Qed.
 
-  Lemma access_elem_in_array: forall a a' E (elem: sep_predicate mem E) vsOld vOld sz,
+  Lemma access_elem_in_array: forall a a' E (elem: sep_predicate mem E) sz fullLength,
       0 < sz < 2 ^ width ->
-      word.unsigned (word.sub a' a) mod sz = 0 ->
       let i := Z.to_nat (word.unsigned (word.sub a' a) / sz) in
-      (* only here to make sure automation picks the right array *)
-      (i < List.length vsOld)%nat ->
-      split_sepclause (a :-> vsOld : array elem (word.of_Z sz)) (a' :-> vOld : elem)
-        (forall vs vs1 v vs2,
-           (* connected with /\ because it needs to be solved by considering both at once *)
-           vs = vs1 ++ [v] ++ vs2 /\ List.length vs1 = i ->
-           iff1 (a :-> vs : array elem (word.of_Z sz))
-                (sep (a' :-> v : elem)
-                     (seps [a :-> vs1 : array elem (word.of_Z sz);
-                            word.add a (word.of_Z (sz * Z.of_nat (S i))) :-> vs2
-                              : array elem (word.of_Z sz)]))).
+      (word.unsigned (word.sub a' a) mod sz = 0 /\
+       (* only here to make sure automation picks the right array *)
+       (i < fullLength)%nat) ->
+      forall vs vs1 v vs2,
+        (* connected with /\ because it needs to be solved by considering both at once *)
+        vs = vs1 ++ [v] ++ vs2 /\ List.length vs1 = i ->
+        iff1 (a :-> vs : array elem (word.of_Z sz))
+             (sep (a' :-> v : elem)
+                  (seps [a :-> vs1 : array elem (word.of_Z sz);
+                         word.add a (word.of_Z (sz * Z.of_nat (S i))) :-> vs2
+                           : array elem (word.of_Z sz)])).
   Proof.
-    unfold split_sepclause.
     unfold sepcl, seps.
     intros. fwd.
     cbn [List.app].
@@ -82,7 +53,7 @@ Section SepLog.
     cbn [Array.array].
     cancel.
     cancel_seps_at_indices 0%nat 0%nat. {
-      f_equal. rewrite H2p1.
+      f_equal. rewrite H1p1.
       destruct width_cases; ZnWords.
     }
     cancel_seps_at_indices 0%nat 0%nat. {
@@ -91,17 +62,19 @@ Section SepLog.
     reflexivity.
   Qed.
 
-  Lemma access_subarray_stmt: forall a a' E (elem: sep_predicate mem E) sz n,
+  Lemma access_subarray: forall a a' E (elem: sep_predicate mem E) sz n fullLength,
       0 < sz < 2 ^ width ->
-      word.unsigned (word.sub a' a) mod sz = 0 ->
       let i := Z.to_nat (word.unsigned (word.sub a' a) / sz) in
-      (forall vs vs1 vs2 vs3,
-          vs = vs1 ++ vs2 ++ vs3 /\ List.length vs1 = i /\ List.length vs2 = n ->
-           iff1 (a :-> vs : array elem (word.of_Z sz))
-                (sep (a' :-> vs2 : array elem (word.of_Z sz))
-                     (seps [a :-> vs1 : array elem (word.of_Z sz);
-                            word.add a (word.of_Z (sz * Z.of_nat (i + n))) :-> vs3
-                              : array elem (word.of_Z sz)]))).
+      (word.unsigned (word.sub a' a) mod sz = 0 /\
+       (* only here to make sure automation picks the right array *)
+       (i + n <= fullLength)%nat) ->
+      forall vs vs1 vs2 vs3,
+        vs = vs1 ++ vs2 ++ vs3 /\ List.length vs1 = i /\ List.length vs2 = n ->
+        iff1 (a :-> vs : array elem (word.of_Z sz))
+             (sep (a' :-> vs2 : array elem (word.of_Z sz))
+                  (seps [a :-> vs1 : array elem (word.of_Z sz);
+                         word.add a (word.of_Z (sz * Z.of_nat (i + n))) :-> vs3
+                           : array elem (word.of_Z sz)])).
   Proof.
     intros.
     unfold sepcl, seps.
@@ -118,70 +91,16 @@ Section SepLog.
     reflexivity.
   Qed.
 
-  (* used when the length of vsPart can be computed with concrete_length *)
-  Lemma access_subarray_concrete_length: forall a a' E (elem: sep_predicate mem E) sz n
-                                                vsAll vsPart,
+  Lemma access_suffix: forall a a' E (elem: sep_predicate mem E) sz lenPrefix,
       0 < sz < 2 ^ width ->
-      word.unsigned (word.sub a' a) mod sz = 0 ->
-      let i := Z.to_nat (word.unsigned (word.sub a' a) / sz) in
-      (* only here to make sure automation picks the right array *)
-      (i + n <= List.length vsAll)%nat ->
-      split_sepclause (a :-> vsAll : array elem (word.of_Z sz))
-                      (a' :-> vsPart : array elem (word.of_Z sz))
-        (forall vs vs1 vs2 vs3,
-           vs = vs1 ++ vs2 ++ vs3 /\ List.length vs1 = i /\ List.length vs2 = n ->
-           iff1 (a :-> vs : array elem (word.of_Z sz))
-                (sep (a' :-> vs2 : array elem (word.of_Z sz))
-                     (seps [a :-> vs1 : array elem (word.of_Z sz);
-                            word.add a (word.of_Z (sz * Z.of_nat (i + n))) :-> vs3
-                              : array elem (word.of_Z sz)]))).
+      word.sub a' a = word.mul (word.of_Z sz) (word.of_Z (Z.of_nat lenPrefix)) ->
+      forall vs vs1 vs2,
+        vs = vs1 ++ vs2 /\ List.length vs1 = lenPrefix ->
+        iff1 (a :-> vs : array elem (word.of_Z sz))
+             (sep (a' :-> vs2 : array elem (word.of_Z sz))
+                  (seps [a :-> vs1 : array elem (word.of_Z sz)])).
   Proof.
-    intros. unfold split_sepclause. intros. eapply access_subarray_stmt; eassumption.
-  Qed.
-
-  Lemma access_subarray_with_len: forall a a' E (elem: sep_predicate mem E) sz n
-                                         vsAll vsPart,
-      0 < sz < 2 ^ width ->
-      word.unsigned (word.sub a' a) mod sz = 0 ->
-      let i := Z.to_nat (word.unsigned (word.sub a' a) / sz) in
-      (* only here to make sure automation picks the right array *)
-      (i + n <= List.length vsAll)%nat ->
-      split_sepclause (a :-> vsAll : array elem (word.of_Z sz))
-                      (a' :-> vsPart : with_len n (array elem (word.of_Z sz)))
-        (forall vs vs1 vs2 vs3,
-           vs = vs1 ++ vs2 ++ vs3 /\ List.length vs1 = i /\ List.length vs2 = n ->
-           iff1 (a :-> vs : array elem (word.of_Z sz))
-                (sep (a' :-> vs2 : with_len n (array elem (word.of_Z sz)))
-                     (seps [a :-> vs1 : array elem (word.of_Z sz);
-                            word.add a (word.of_Z (sz * Z.of_nat (i + n))) :-> vs3
-                              : array elem (word.of_Z sz)]))).
-  Proof.
-    intros. unfold split_sepclause. intros.
-    unfold with_len, with_pure, sepcl. fwd.
-    replace (length vs2 = length vs2) with True. 2: {
-      eapply PropExtensionality.propositional_extensionality. split; auto.
-    }
-    etransitivity.
-    1: eapply access_subarray_stmt; eauto.
-    unfold sepcl.
-    cbn [seps]. ecancel.
-  Qed.
-
-  Lemma access_suffix: forall a a' E (elem: sep_predicate mem E) sz vsPrefix vsSuffix,
-      0 < sz < 2 ^ width ->
-      word.sub a' a = word.mul (word.of_Z sz)
-                               (word.of_Z (Z.of_nat (List.length vsPrefix))) ->
-      split_sepclause (a :-> List.app vsPrefix vsSuffix : array elem (word.of_Z sz))
-                      (a' :-> vsSuffix : array elem (word.of_Z sz))
-        (forall vs vs1 vs2,
-           vs = vs1 ++ vs2 /\
-           List.length vs1 = List.length vsPrefix /\
-           List.length vs2 = List.length vsSuffix ->
-           iff1 (a :-> vs : array elem (word.of_Z sz))
-                (sep (a' :-> vs2 : array elem (word.of_Z sz))
-                     (seps [a :-> vs1 : array elem (word.of_Z sz)]))).
-  Proof.
-    intros. unfold split_sepclause. intros. fwd.
+    intros. intros. fwd.
     rewrite array_app. cbn [seps].
     cancel. cbn [seps].
     match goal with
@@ -191,17 +110,15 @@ Section SepLog.
     destruct width_cases; ZnWords.
   Qed.
 
-  Lemma access_tail: forall a a' E (elem: sep_predicate mem E) sz vH vsTail,
+  Lemma access_tail: forall a a' E (elem: sep_predicate mem E) sz,
       0 < sz < 2 ^ width ->
       word.sub a' a = word.of_Z sz ->
-      split_sepclause (a :-> List.cons vH vsTail : array elem (word.of_Z sz))
-                      (a' :-> vsTail : array elem (word.of_Z sz))
-        (forall v vs,
-            iff1 (a :-> List.cons v vs : array elem (word.of_Z sz))
-                 (sep (a' :-> vs : array elem (word.of_Z sz))
-                      (seps [a :-> v : elem]))).
+      forall v vs,
+        iff1 (a :-> List.cons v vs : array elem (word.of_Z sz))
+             (sep (a' :-> vs : array elem (word.of_Z sz))
+                  (seps [a :-> v : elem])).
   Proof.
-    intros. unfold split_sepclause. intros. unfold sepcl. cbn.
+    intros. intros. unfold sepcl. cbn.
     cancel. cbn [seps].
     match goal with
     | |- iff1 (Array.array _ _ ?x _) _ => replace x with a'
@@ -322,33 +239,38 @@ Ltac concrete_sz_bounds :=
 
 (* split_sepclause_goal: *)
 
-#[export] Hint Extern 1 (split_sepclause (_ :-> _ : array ?elem ?sz) (_ :-> _ : ?elem) _) =>
-  eapply access_elem_in_array; [ concrete_sz_bounds | listZnWords | listZnWords ]
+#[export] Hint Extern 1
+  (split_sepclause (?a :-> ?vsAll : array ?elem (word.of_Z ?sz)) (?a' :-> _ : ?elem) _ _) =>
+  unshelve (epose proof (access_elem_in_array a a' _ elem sz (List.length vsAll) _ _));
+  [ concrete_sz_bounds | listZnWords | shelve ]
 : split_sepclause_goal.
 
 #[export] Hint Extern 1
-  (split_sepclause (?a :-> ?vsAll : array ?elem ?sz)
-                   (?a' :-> ?vsPart : with_len ?n (array ?elem ?sz)) _) =>
-  eapply (access_subarray_with_len a a' _ elem _ n vsAll vsPart);
-  [ concrete_sz_bounds | listZnWords | listZnWords ]
+  (split_sepclause (?a :-> ?vsAll : array ?elem (word.of_Z ?sz))
+                   (?a' :-> ?vsPart : array ?elem (word.of_Z ?sz)) _ ?G) =>
+  (* most likely, vsPart is still an evar (because it's universally quantified by the
+     callee's correctness lemma), so we have to search for its desired length in G,
+     but maybe it has a concrete structure (eg [?a; ?b; ?c]), in which case
+     concrete_list_length can find that length *)
+  let n := match G with
+           | _ /\ ?C => match C with context[List.length vsPart = ?n] => n end
+           | _ => concrete_list_length vsPart
+           end in
+  unshelve (epose proof (access_subarray a a' _ elem sz n (List.length vsAll) _ _));
+  [ concrete_sz_bounds | listZnWords | shelve ]
+: split_sepclause_goal.
+
+#[export] Hint Extern 1 (split_sepclause (?a  :-> ?vs1 ++ ?vs2 : array ?elem (word.of_Z ?sz))
+                                         (?a' :-> ?vs2 : array ?elem (word.of_Z ?sz)) _ _) =>
+  unshelve (epose proof (access_suffix a a' _ elem sz (List.length vs1) _ _));
+  [ concrete_sz_bounds | listZnWords | shelve ]
 : split_sepclause_goal.
 
 #[export] Hint Extern 1
-  (split_sepclause (?a :-> ?vsAll : array ?elem ?sz)
-                   (?a' :-> ?vsPart : array ?elem ?sz) _) =>
-  let n := concrete_list_length vsPart in
-  eapply (access_subarray_concrete_length a a' _ elem _ n vsAll vsPart);
-  [ concrete_sz_bounds | listZnWords | listZnWords ]
-: split_sepclause_goal.
-
-#[export] Hint Extern 1 (split_sepclause (_ :-> ?vs1 ++ ?vs2 : array ?elem ?sz)
-                                         (_ :-> ?vs2 : array ?elem ?sz) _) =>
-  eapply access_suffix; [ concrete_sz_bounds | listZnWords ]
-: split_sepclause_goal.
-
-#[export] Hint Extern 1 (split_sepclause (_ :-> (_ :: ?vsTail) : array ?elem ?sz)
-                                         (_ :-> ?vsTail : array ?elem ?sz) _) =>
-  eapply access_tail; [ concrete_sz_bounds | listZnWords ]
+  (split_sepclause (?a  :-> (_ :: ?vsTail) : array ?elem (word.of_Z ?sz))
+                   (?a' :-> ?vsTail : array ?elem (word.of_Z ?sz)) _ _) =>
+  unshelve (epose proof (access_tail a a' _ elem sz _ _));
+  [ concrete_sz_bounds | listZnWords | shelve ]
 : split_sepclause_goal.
 
 
